extract RakeMap.lean; fix project errors

Rake.lean
@@ -17,6 +17,12 @@ structure Rake : Type where
   hsort : sorted → List.Sorted (·<·) ks := by simp
   hsize : 0 < ks.length := by simp
 
+namespace Rake
+
+def zer : Rake := { d := 0, ks := [0] }
+def nat : Rake := { d := 1, ks := [0] }
+def ge2 : Rake := { d := 1, ks := [2] }
+
 def sort_nodup (xs:List Nat) (hxs₀ : List.Nodup xs)
 : { xs':List Nat // List.Sorted (·<·) xs' ∧ xs'.length = xs.length } :=
   let xs' := xs.mergeSort (·≤·)
@@ -25,16 +31,12 @@ def sort_nodup (xs:List Nat) (hxs₀ : List.Nodup xs)
   have hlength := by simp_all only [List.length_mergeSort, xs']
   ⟨xs', And.intro (List.Sorted.lt_of_le hsorted hnodup) hlength⟩
 
-def zer : Rake := { d := 0, ks := [0] }
-def nat : Rake := { d := 1, ks := [0] }
-def ge2 : Rake := { d := 1, ks := [2] }
-
-def Rake.term (r: Rake) (n : Nat) : Nat :=
+def term (r: Rake) (n : Nat) : Nat :=
   let q := r.ks.length
   have : n%q < r.ks.length := Nat.mod_lt _ r.hsize
   aseq r.ks[n%q] r.d |>.term (n/q)
 
-def Rake.sort (r: Rake) : {r':Rake // r'.sorted } :=
+def sort (r: Rake) : {r':Rake // r'.sorted } :=
   if h: r.sorted then ⟨r, h⟩
   else
     let ks₀ := r.ks
@@ -50,15 +52,15 @@ lemma length_pos_of_dedup {l:List Nat} (hlen: 0 < l.length) : 0 < l.dedup.length
   rw[←List.mem_dedup] at this
   exact List.length_pos_of_mem this
 
-def Rake.gte (r: Rake) (n: Nat) : Rake  :=
+def gte (r: Rake) (n: Nat) : Rake  :=
   let f : ℕ → ℕ := (λk => let s := aseq k r.d; (ASeq.gte s n).k)
   { d := r.d, ks := r.ks.map f, sorted := false,
     hsize := Nat.lt_of_lt_of_eq r.hsize (r.ks.length_map _).symm }
 
-def Rake.seq (r:Rake) (n:Nat) {hn:n<r.ks.length} : ASeq :=
+def seq (r:Rake) (n:Nat) {hn:n<r.ks.length} : ASeq :=
   aseq (r.ks[n]'hn) r.d
 
-def Rake.seqs (r: Rake) : List ASeq :=
+def seqs (r: Rake) : List ASeq :=
   r.ks.map (λ k => aseq k r.d)
 
 /--
@@ -66,7 +68,7 @@ Partition each sequence in the rake by partitioning their *inputs*
 into equivalance classes mod n. This multiplies the number of sequences
 by n. We can't allow n to be zero because then we'd have no sequences left,
 and this would break the guarantee that term (n) < term n+1. -/
-def Rake.partition (r: Rake) (n: Nat) (hn: 0 < n): Rake :=
+def partition (r: Rake) (n: Nat) (hn: 0 < n): Rake :=
   let seqs' := r.seqs.map (λ s => s.partition n) |>.join
   let ks₀ := seqs'.map (λ s => s.k)
   -- aseq.partiton n  always produces a list of length n
@@ -87,7 +89,7 @@ def Rake.partition (r: Rake) (n: Nat) (hn: 0 < n): Rake :=
     aesop
   { d := r.d * n, ks := ks₀, sorted := false, hsize := hsize }
 
-def Rake.rem (r : Rake) (n : Nat) : Rake :=
+def rem (r : Rake) (n : Nat) : Rake :=
   if hn₀ : n = 0 then r.gte 1
   else
     have hn : 0 < n := Nat.zero_lt_of_ne_zero hn₀
@@ -100,7 +102,7 @@ def Rake.rem (r : Rake) (n : Nat) : Rake :=
 
 /-- proof that if a rake produces a term, it's because one of the sequences
     it contains produces that term. -/
-lemma Rake.___unused______ex_seq (r: Rake)
+lemma ___unused______ex_seq (r: Rake)
   : (r.term m = n) → (∃k ∈ r.ks, n = k + r.d * (m/r.ks.length)) := by
   unfold term; intro hmn; simp_all
   let q := r.ks.length
@@ -120,7 +122,7 @@ theorem div_lt_of_lt_mod_eq {m n d:Nat} {hdpos: 0 < d} {hmn: m<n} : (m%d = n%d) 
   rw[←m.div_add_mod d, ←n.div_add_mod d, hmod, Nat.add_lt_add_iff_right] at hmn
   exact (Nat.mul_lt_mul_left hdpos).mp hmn
 
-theorem Rake.term_simp (r:Rake) (n:Nat)
+theorem term_simp (r:Rake) (n:Nat)
 : (∃k, (r.term n = k + r.d * (n/r.ks.length)) ∧ ∃i: Fin r.ks.length, i=n%r.ks.length ∧ k=r.ks[i]) := by
   let i: Fin r.ks.length := ⟨n%r.ks.length, Nat.mod_lt n r.hsize⟩
   use r.ks[i]
@@ -128,7 +130,7 @@ theorem Rake.term_simp (r:Rake) (n:Nat)
   · dsimp[term, aseq, ASeq.term, i]
   · use i
 
-theorem Rake.term_iff (r:Rake)
+theorem term_iff (r:Rake)
   : ∀m, (∃n, r.term n = m) ↔ (∃ k∈r.ks,  ∃x:Nat, k+x*r.d = m) := by
   intro m; apply Iff.intro
   · show (∃ n, r.term n = m) → ∃ k ∈ r.ks, ∃ x, k + x * r.d = m
@@ -184,7 +186,7 @@ As currently defined, the terms of a sorted rake can be non-ascending in one of 
 - ascending sawtooth pattern if ∃k∈r.ks, k>r.d
 - cyclic (and possibly constant) if r.d=0
 But in all cases, if the rake is sorted, term 0 is the minimum. -/
-theorem Rake.sorted_min_term_zero (r: Rake) (hr: r.sorted) : ∀ n, (r.term 0 ≤ r.term n) := by
+theorem sorted_min_term_zero (r: Rake) (hr: r.sorted) : ∀ n, (r.term 0 ≤ r.term n) := by
   intro n
   obtain ⟨k₀, hk₀, i₀, hi₀⟩ := r.term_simp 0
   obtain ⟨k₁, hk₁, i₁, hi₁⟩ := r.term_simp n
@@ -196,70 +198,3 @@ theorem Rake.sorted_min_term_zero (r: Rake) (hr: r.sorted) : ∀ n, (r.term 0 �
   case zlt =>
     have : i₀.val < i₁.val := by aesop
     exact Nat.le_of_succ_le <| sorted_get r.ks (r.hsort hr) i₀ i₁ this
-
--- rakemap --------------------------------------------------------------------
-
-structure RakeMap (pred: Nat → Prop) where
-  rake : Rake
-  hbij : ∀ n, pred n ↔ ∃ m, rake.term m = n
-
-def RakeMap.pred {p:Nat → Prop} (_:RakeMap p) : Nat → Prop := p
-
-/-- proof that rm_nat.term provides a bijection from Nat → Nat
- (it happens to be an identity map, but this is not necessary for proofs) -/
-def rm_nat : RakeMap (λ _ => True) := {
-  rake := nat
-  hbij := by intro n; simp[Rake.term, nat, aseq, ASeq.term]}
-
-def rm_ge2 : RakeMap (λn => 2≤n) := {
-  rake := ge2
-  hbij := by
-    intro n; simp[Rake.term, ge2, aseq, ASeq.term]; apply Iff.intro
-    · show 2 ≤ n → ∃ m, 2 + m = n
-      intro n2; use n-2; simp_all
-    · show (∃ m, 2 + m = n) → 2 ≤ n
-      intro hm; obtain ⟨m,hm⟩ := hm; rw[←hm]; simp }
-
-section rem_lemmas
-
-  -- now it's more complicated. first we partition each sequence
-  -- then we remove the sequences that are multiples of a prime
-  -- how do we know:
-  --   - we dropped the multiples?
-  --     - partition step keeps same terms
-  --     - but now every sequence either ALWAYS or NEVER produces multiples of p
-  --     - we can tell the difference, and only drop the ones that always produce multiples
-  --   - we know we kept everything else because it's a straight filter operation.
-
-
-  variable (rm: RakeMap prop) (p n: Nat) {hp: 0<p}
-
-  lemma RakeMap.rem_drop -- rem drops multiples of p
-    : p∣n → ¬(∃m, (rm.rake.rem p).sort.val.term m = n) := by
-    sorry
-
-  lemma RakeMap.rem_keep -- rem keeps non-multiples of p
-    : ¬(p∣n) ∧ (∃pm, rm.rake.term pm = n) → (∃m, (rm.rake.rem p).sort.val.term m = n) := by
-    sorry
-
-  lemma RakeMap.rem_same -- rem introduces no new terms
-    : (∃m, (rm.rake.rem p).sort.val.term m = n) → (∃pm, rm.rake.term pm = n) := by
-    sorry
-
-end rem_lemmas
-
--- operations on RakeMap -------------------------------------------------------
-
-def RakeMap.rem (prev : RakeMap prop) (p: Nat)
-  : RakeMap (λ n => prop n ∧ ¬(p∣n)) :=
-  let rake := (prev.rake.rem p).sort
-  let proof := by
-    intro n; symm
-    let hm : Prop := (∃m, rake.val.term m = n)
-    let hpm : Prop := (∃pm, prev.rake.term pm = n )
-    have : prop n ↔ hpm := prev.hbij n
-    have : p∣n → ¬hm := rem_drop prev p n
-    have : ¬p∣n ∧ hpm → hm := rem_keep prev p n
-    have : hm → hpm := rem_same prev p n
-    by_cases p∣n; all_goals aesop
-  { rake := rake, hbij := proof }
