lakefile.lean
@@ -8,6 +8,7 @@ lean_lib PrimeGen { }
 lean_lib PrimeSieve { }
 lean_lib ASeq { }
 lean_lib Rake { }
+lean_lib RakeMap { }
 lean_lib RakeSieve { }
 
 @[default_target]
